theories/clang/tactics.v
@@ -4,25 +4,17 @@ Require Import lib.gmap_solve.
 Set Default Proof Using "Type".
 Import uPred.
 
-Ltac solve_typeof :=
-  match goal with
-    | |- typeof _ (Vint32 _) => apply typeof_int32
-    | |- typeof _ (Vint8 _) => apply typeof_int8
-    | |- typeof Tnull Vnull => apply typeof_null
-    | |- typeof _ Vnull => apply typeof_null_ptr
-    | |- typeof (Tptr _) (Vptr _) => apply typeof_ptr
-  end.
-
-Lemma typeof_any_ptr (t1 t2: type) (v: val):
-  typeof (Tptr t1) v → typeof (Tptr t2) v.
-Proof.
-  induction v; intros H; try (inversion H); try solve_typeof.
-Qed.
-
 Ltac wp_done :=
   match goal with
-  | |- typeof _ _ => solve_typeof
-  | _ => fast_done
+    | |- typeof _ _ => (fast_done || constructor)
+    | |- assign_type_compatible _ _ => (fast_done || constructor)
+    | _ => fast_done
+  end.
+
+Ltac solve_assign_type t :=
+  match t with
+    | Tptr ?t' => (apply (assign_ptr_ptr t') || apply (assign_null_ptr t'))
+    | _ => constructor
   end.
 
 (** The tactic [reshape_expr e tac] decomposes the expression [e] into an
@@ -35,22 +27,9 @@ Ltac reshape_expr e tac :=
   | _ => tac (reverse K) e
   | Ebinop ?op (Evalue ?v1) ?e2 => go (EKbinopl op v1 :: K) e2
   | Ebinop ?op ?e1 ?e2 => go (EKbinopr op e2 :: K) e1
-  (* | If ?e0 ?e1 ?e2 => go (IfCtx e1 e2 :: K) e0 *)
-  (* | Pair ?e1 ?e2 => reshape_val e1 ltac:(fun v1 => go (PairRCtx v1 :: K) e2) *)
-  (* | Pair ?e1 ?e2 => go (PairLCtx e2 :: K) e1 *)
   | Efst ?e => go (EKfst :: K) e
   | Esnd ?e => go (EKsnd :: K) e
-  (* | InjL ?e => go (InjLCtx :: K) e *)
-  (* | InjR ?e => go (InjRCtx :: K) e *)
-  (* | Case ?e0 ?e1 ?e2 => go (CaseCtx e1 e2 :: K) e0 *)
-  (* | Alloc ?e => go (AllocCtx :: K) e *)
   | Ederef ?e => go (EKderef :: K) e
-  (* | Store ?e1 ?e2 => reshape_val e1 ltac:(fun v1 => go (StoreRCtx v1 :: K) e2) *)
-  (* | Store ?e1 ?e2 => go (StoreLCtx e2 :: K) e1 *)
-  (* | CAS ?e0 ?e1 ?e2 => reshape_val e0 ltac:(fun v0 => first *)
-  (*    [ reshape_val e1 ltac:(fun v1 => go (CasRCtx v0 v1 :: K) e2) *)
-  (*    | go (CasMCtx v0 e2 :: K) e1 ]) *)
-  (* | CAS ?e0 ?e1 ?e2 => go (CasLCtx e1 e2 :: K) e0 *)
   end in go (@nil exprctx) e.
 
 Ltac reshape_stmts s tac :=
@@ -62,22 +41,6 @@ Ltac reshape_stmts s tac :=
     | Swhile ?c ?e ?s =>
       reshape_expr e ltac:(fun Kes e' => tac Kes (SKwhile c s) e')
   end.
-
-(* Ltac wp_bind_e_core K := *)
-(*   lazymatch eval hnf in K with *)
-(*   | [] => idtac *)
-(*   | _ => etrans; [|fast_by apply (wp_bind_e K)]; simpl *)
-(*   end. *)
-
-(* Tactic Notation "wp_bind_e" open_constr(efoc) := *)
-(*   iStartProof; *)
-(*   lazymatch goal with *)
-(*   | |- _ ⊢ wp ?E (cure ?e) ?Q ?P => reshape_expr e ltac:(fun K e' => *)
-(*     match e' with *)
-(*     | efoc => unify e' efoc; wp_bind_e_core K *)
-(*     end) || fail "wp_bind_e: cannot find" efoc "in" e *)
-(*   | _ => fail "wp_bind_e: not a 'wp'" *)
-(*   end. *)
 
 Ltac wp_bind_core Kes Ks :=
   lazymatch eval hnf in Kes with
@@ -99,24 +62,39 @@ Tactic Notation "wp_bind" open_constr(efoc) :=
 Section heap.
 Context `{clangG Σ}.
 
-Lemma tac_wp_assign Δ Δ' Δ'' E i l (v v': val) Φ Φret:
-  same_size v v' →
+Lemma tac_wp_assign Δ Δ' Δ'' E i l (v v': val) (t t': type) Φ Φret:
+  typeof v' t' → assign_type_compatible t t' →
   IntoLaterNEnvs 1 Δ Δ' →
-  envs_lookup i Δ' = Some (false, l ↦ v)%I →
-  envs_simple_replace i false (Esnoc Enil i (l ↦ v')) Δ' = Some Δ'' →
+  envs_lookup i Δ' = Some (false, l ↦ v @ t)%I →
+  envs_simple_replace i false (Esnoc Enil i (l ↦ v' @ t)) Δ' = Some Δ'' →
   (Δ'' ⊢ Φ Vvoid) →
   Δ ⊢ WP curs (Sassign (Evalue (Vptr l)) (Evalue v')) @ E {{ Φ ; Φret }}.
 Proof.
   intros. eapply wand_apply.
-  { iIntros "HP HQ". iApply wp_assign; first done.
+  { iIntros "HP HQ". iApply wp_assign; [done|done|].
     iSplitL "HP"; eauto. }
   rewrite into_laterN_env_sound -later_sep envs_simple_replace_sound //; simpl.
   rewrite right_id. apply later_mono, sep_mono_r, wand_mono=>//.
 Qed.
 
-Lemma tac_wp_load Δ Δ' E i l q v Φ Φret:
+Lemma tac_wp_assign_offset Δ Δ' Δ'' E i b (o off: nat) (v1 v2 v2': val) (t1 t2 t2': type) Φ Φret:
+  typeof v2' t2' → assign_type_compatible t2 t2' → sizeof t1 = off →
   IntoLaterNEnvs 1 Δ Δ' →
-  envs_lookup i Δ' = Some (false, l ↦{q} v)%I →
+  envs_lookup i Δ' = Some (false, (b, o) ↦ Vpair v1 v2 @ Tprod t1 t2)%I →
+  envs_simple_replace i false (Esnoc Enil i ((b, o) ↦ Vpair v1 v2' @ Tprod t1 t2)) Δ' = Some Δ'' →
+  (Δ'' ⊢ Φ Vvoid) →
+  Δ ⊢ WP curs (Sassign (Evalue (Vptr (b, (o + off)%nat))) (Evalue v2')) @ E {{ Φ ; Φret }}.
+Proof.
+  intros. eapply wand_apply.
+  { iIntros "HP HQ". iApply wp_assign_offset; [done|done|done|].
+    iSplitL "HP"; eauto. }
+  rewrite into_laterN_env_sound -later_sep envs_simple_replace_sound //; simpl.
+  rewrite right_id. apply later_mono, sep_mono_r, wand_mono=>//.
+Qed.
+
+Lemma tac_wp_load Δ Δ' E i l q v t Φ Φret:
+  IntoLaterNEnvs 1 Δ Δ' →
+  envs_lookup i Δ' = Some (false, l ↦{q} v @ t)%I →
   (Δ' ⊢ Φ v) →
   Δ ⊢ WP (cure (Ederef (Evalue (Vptr l)))) @ E {{ Φ ; Φret }}.
 Proof.
@@ -132,15 +110,31 @@ Tactic Notation "wp_assign" :=
   iStartProof;
   try (iApply wp_seq);
   lazymatch goal with
-  | |- _ ⊢ wp ?E (curs (Sassign ?e _)) ?P ?Q =>
-    eapply tac_wp_assign;
-      [let v := match goal with |- typeof ?t ?v => v end in
-       wp_done || fail "wp_store:" v "doesn't type check"
-      |apply _
-      |let l := match goal with |- _ = Some (_, (?l ↦{_} _)%I) => l end in
-       iAssumptionCore || fail "wp_assign: cannot find" l "↦ ?"
-      |env_cbv; reflexivity
-      | auto (* wp_finish *)]
+  | |- _ ⊢ wp ?E (curs (Sassign (Evalue (Vptr (?b, (?o + ?off)%nat))) _)) ?P ?Q =>
+    iMatchHyp (fun H P => match P with ((b, o) ↦{_} _ @ ?t)%I =>
+      eapply tac_wp_assign_offset;
+        [let v := match goal with |- typeof ?t ?v => v end in
+         wp_done || fail "wp_store:" v "doesn't type check"
+        |solve_assign_type t || fail "wp_assign: assignment types are not compatible"
+        |idtac (* XXX *)
+        |apply _
+        |let l := match goal with |- _ = Some (_, (?l ↦{_} _ @ _)%I) => l end in
+         iAssumptionCore || fail "wp_assign: cannot find" l "↦ ?"
+        |env_cbv; reflexivity
+        | auto (* wp_finish *)]
+    end)
+  | |- _ ⊢ wp ?E (curs (Sassign (Evalue (Vptr ?l)) _)) ?P ?Q =>
+    iMatchHyp (fun H P => match P with (l ↦{_} _ @ ?t)%I =>
+      eapply tac_wp_assign;
+        [let v := match goal with |- typeof ?t ?v => v end in
+         wp_done || fail "wp_store:" v "doesn't type check"
+        |solve_assign_type t || fail "wp_assign: assignment types are not compatible"
+        |apply _
+        |let l := match goal with |- _ = Some (_, (?l ↦{_} _ @ _)%I) => l end in
+         iAssumptionCore || fail "wp_assign: cannot find" l "↦ ?"
+        |env_cbv; reflexivity
+        | auto (* wp_finish *)]
+    end)
   | _ => fail "wp_assign: not a 'wp'"
   end.
 
@@ -155,7 +149,7 @@ Tactic Notation "wp_load" :=
       |fail 1 "wp_load: cannot find 'Ederef' in" s];
     eapply tac_wp_load;
       [apply _
-      |let l := match goal with |- _ = Some (_, (?l ↦{_} _)%I) => l end in
+      |let l := match goal with |- _ = Some (_, (?l ↦{_} _ @ _)%I) => l end in
        iAssumptionCore || fail "wp_load: cannot find" l "↦ ?"
       |(* wp_finish *) auto]
   | _ => fail "wp_load: not a 'wp'"
